Progress on axiom 1

theories/interval.v
@@ -14,7 +14,7 @@ Definition yoᶠ (l : ℙ) {p} : @El p Typeᶠ.
 Proof.
 unshelve refine (fun q α => mkTYPE _ _ _).
 + unshelve refine (fun r β => r ≤ l).
-+ unshelve refine (fun f => yoR l q f). 
++ unshelve refine (fun f => yoR l q f).
 Defined.
 
 Definition yoε (l : ℙ) {p : ℙ} : @Elε p Typeᶠ Typeε (yoᶠ l).
@@ -23,10 +23,28 @@ unfold Elε; cbn.
 reflexivity.
 Defined.
 
-(* Interval with endpoints *)
+(* Interval *)
 
 Definition Iᶠ {p} : @El p Typeᶠ := yoᶠ 1.
 Definition Iε {p} : @Elε p Typeᶠ Typeε Iᶠ := yoε 1.
+
+Definition seq_I {p : ℙ}
+    {i : @El p Iᶠ} {iε : Elε Iᶠ Iε i}
+    {j : @El p Iᶠ} {jε : Elε Iᶠ Iε j} :
+    i p ! ≡ j p ! -> i ≡ j.
+Proof.
+intro H.
+pose proof (iε p !) as Hi. inversion Hi as [α Hα].
+cbn in Hα. change (! · i) with i in Hα.
+pose proof (jε p !) as Hj. inversion Hj as [β Hβ].
+cbn in Hβ. change (! · j) with j in Hβ.
+rewrite <- Hα. rewrite <- Hβ.
+rewrite <- Hα in H. change (α ∘ !) with α in H.
+rewrite <- Hβ in H. change (β ∘ !) with β in H.
+destruct H. refine (srefl _).
+Defined.
+
+(* Interval endpoint i0 *)
 
 Definition cst_0 (p : ℙ) : p ≤ 1.
 Proof.
@@ -45,6 +63,8 @@ Proof.
 refine (fun q α => yoR_cons 1 q (cst_0 q)).
 Defined.
 
+(* Interval endpoint i1 *)
+
 Definition cst_1 (p : ℙ) : p ≤ 1.
 Proof.
 unshelve refine (mkCubeArr _ _ _ _).
@@ -62,7 +82,136 @@ Proof.
 refine (fun q α => yoR_cons 1 q (cst_1 q)).
 Defined.
 
-(* Axioms on the interval *)
+(* Axiom 1 : the interval is connected *)
+
+Definition isdecᶠ {p : ℙ}
+    (φ : @El p (Arr Iᶠ Iε Typeᶠ Typeε))
+    (φε : Elε _ (Arrε Iᶠ Iε Typeᶠ Typeε) φ) :
+    @El p (Arr Iᶠ Iε Typeᶠ Typeε) :=
+(lamᶠ (fun q α i iε =>
+    sumᶠ (appᶠ (α · φ) i iε) (appε (α · φε) i iε)
+         (Arr _ (appε (α · φε) i iε) emptyᶠ emptyε)
+         (Arrε (appᶠ (α · φ) i iε) (appε (α · φε) i iε) emptyᶠ emptyε))).
+
+Definition isdecε {p : ℙ}
+    (φ : @El p (Arr Iᶠ Iε Typeᶠ Typeε))
+    (φε : Elε _ (Arrε Iᶠ Iε Typeᶠ Typeε) φ) :
+    Elε _ (Arrε Iᶠ Iε Typeᶠ Typeε) (isdecᶠ φ φε) :=
+(lamε (fun q α i iε =>
+    sumε (appᶠ (α · φ) i iε) (appε (α · φε) i iε)
+         (Arr _ (appε (α · φε) i iε) emptyᶠ emptyε)
+         (Arrε (appᶠ (α · φ) i iε) (appε (α · φε) i iε) emptyᶠ emptyε))).
+
+Definition negᶠ {p : ℙ}
+    (φ : @El p (Arr Iᶠ Iε Typeᶠ Typeε))
+    (φε : Elε _ (Arrε Iᶠ Iε Typeᶠ Typeε) φ) :
+    @El p (Arr Iᶠ Iε Typeᶠ Typeε) :=
+(lamᶠ (fun q α i iε =>
+    Arr (appᶠ (α · φ) i iε) (appε (α · φε) i iε)
+        emptyᶠ emptyε)).
+
+Definition negε {p : ℙ}
+    (φ : @El p (Arr Iᶠ Iε Typeᶠ Typeε))
+    (φε : Elε _ (Arrε Iᶠ Iε Typeᶠ Typeε) φ) :
+    Elε _ (Arrε Iᶠ Iε Typeᶠ Typeε) (negᶠ φ φε) :=
+(lamε (fun q α i iε =>
+    Arrε (appᶠ (α · φ) i iε) (appε (α · φε) i iε)
+        emptyᶠ emptyε)).
+
+Definition hot_aux {p : ℙ}
+    (i : @El p Iᶠ) (iε : Elε Iᶠ Iε i) :
+    S p ≤ 1.
+Proof.
+unshelve refine (mkCubeArr _ _ _ _).
+- unshelve refine (fun c => if (c finzero) then _ else _).
+  + refine ((i p !).(arr) (fun n => c (finsucc n))).
+  + refine (fun _ => false).
+- intros c d Hcd.
+  remember (c finzero) as c0. remember (d finzero) as d0.
+  destruct c0 ; destruct d0.
+  + apply ((i p !).(eps_arr)).
+    intro n. exact (Hcd (finsucc n)).
+  + specialize (Hcd finzero).
+    rewrite <- Heqc0 in Hcd. rewrite <- Heqd0 in Hcd. destruct Hcd.
+  + easy.
+  + easy.
+Defined.
+
+Definition homotopy_to_0ᶠ {p : ℙ}
+    (i : @El p Iᶠ) (iε : Elε Iᶠ Iε i) :
+    @El (S p) Iᶠ.
+Proof.
+unshelve refine (fun q α => (hot_aux i iε) ∘ α).
+Defined.
+
+Definition homotopy_to_0ε {p : ℙ}
+    (i : @El p Iᶠ) (iε : Elε Iᶠ Iε i) :
+    Elε Iᶠ Iε (homotopy_to_0ᶠ i iε).
+Proof.
+unshelve refine (fun q α => _).
+refine (yoR_cons 1 q (hot_aux i iε ∘ α)).
+Defined.
+
+Definition side_0 {p : ℙ} : p ≤ S p.
+Proof.
+unshelve refine (mkCubeArr _ _ _ _).
+- unshelve refine (fun c n => _).
+  destruct n as [n nε]. destruct n as [|n'].
+  + exact false.
+  + apply c. unshelve refine (mkFinset p n' _).
+    apply le_to_sle. apply le_S_n. apply sle_to_le. exact nε.
+- intros c d Hcd n. destruct n as [n nε]. destruct n.
+  + exact sI.
+  + refine (Hcd _).
+Defined.
+
+Definition side_1 {p : ℙ} : p ≤ S p.
+Proof.
+unshelve refine (mkCubeArr _ _ _ _).
+- unshelve refine (fun c n => _).
+  destruct n as [n nε]. destruct n as [|n'].
+  + exact true.
+  + apply c. unshelve refine (mkFinset p n' _).
+    apply le_to_sle. apply le_S_n. apply sle_to_le. exact nε.
+- intros c d Hcd n. destruct n as [n nε]. destruct n.
+  + exact sI.
+  + refine (Hcd _).
+Defined.
+
+Definition restriction_0 {p : ℙ}
+{i : @El p Iᶠ} {iε : Elε Iᶠ Iε i} :
+    side_0 · (homotopy_to_0ᶠ i iε) ≡ i0ᶠ.
+Proof.
+apply (@seq_I p (side_0 · homotopy_to_0ᶠ i iε) (side_0 · homotopy_to_0ε i iε) i0ᶠ i0ε).
+apply seq_cube_arr. refine (srefl _).
+Defined.
+
+Definition restriction_1 {p : ℙ}
+    {i : @El p Iᶠ} {iε : Elε Iᶠ Iε i} :
+    side_1 · (homotopy_to_0ᶠ i iε) ≡ i.
+Proof.
+apply (@seq_I p (side_1 · homotopy_to_0ᶠ i iε) (side_1 · homotopy_to_0ε i iε) i iε).
+apply seq_cube_arr. refine (srefl _).
+Defined.
+
+Definition ax1ᶠ {p : ℙ}
+    (φ : @El p (Arr Iᶠ Iε Typeᶠ Typeε))
+    (φε : Elε _ (Arrε Iᶠ Iε Typeᶠ Typeε) φ)
+    (Hφ : @El p (Prod Iᶠ Iε (isdecᶠ φ φε) (isdecε φ φε)))
+    (Hφε : Elε _ (Prodε Iᶠ Iε (isdecᶠ φ φε) (isdecε φ φε)) Hφ) :
+    @El p (sumᶠ (Prod Iᶠ Iε φ φε) (Prodε Iᶠ Iε φ φε)
+                (Prod Iᶠ Iε (negᶠ φ φε) (negε φ φε))
+                (Prodε Iᶠ Iε (negᶠ φ φε) (negε φ φε))).
+Proof.
+unshelve refine (fun q α => _).
+pose proof (Hφ q α (α · i0ᶠ) (α · i0ε)) as H. destruct H as [Hi0 Hi0ε | Hi0 Hi0ε].
+- unshelve refine (inl_ _ _ _ _ _ _).
+  + unshelve refine (fun r β i iε => _).
+    (* pose proof (Hφ r (α ∘ β) (homotopy_to_0ᶠ i iε) (homotopy_to_0ε i iε)) as Hh. *)
+Admitted.
+
+(* Axiom 2 *)
+
 Definition ax2ᶠ {p : ℙ}
     (e : @El p (eqᶠ Iᶠ Iε i0ᶠ i0ε i1ᶠ i1ε))
     (eε : Elε _ (eqε Iᶠ Iε i0ᶠ i0ε i1ᶠ i1ε) e) :
